src/Narcissus/Examples/NetworkStack/IPv4Header.v
@@ -152,6 +152,8 @@ Qed.
 Hint Resolve IPv4_Packet_Header_Len_eq : data_inv_hints.
 Hint Resolve IPv4_Packet_Header_Len_bound : data_inv_hints.
 
+Arguments andb : simpl never.
+
 (* Step Three: Synthesize a decoder and a proof that /it/ is correct. *)
 Definition IPv4_Packet_Header_decoder
   : CorrectAlignedDecoderFor IPv4_Packet_OK IPv4_Packet_Format.
@@ -189,7 +191,7 @@ Definition bin_pkt : Vector.t (word 8) _ :=
 Definition bin_pkt' : Vector.t (word 8) _ :=
   Eval compute in Vector.map (@natToWord 8) [69;0;100;0;0;0;0;0;38;1;0;0;192;168;222;10;192;168;222;1;0;0;0;0].
 
-(* An source version of a packet. *)
+(* An source version of a packet, different from binary packet above. *)
 Definition pkt :=
   {| TotalLength := WO~0~1~1~1~0~1~0~0~0~0~0~0~0~0~0~0;
      ID := wones _;
@@ -221,15 +223,6 @@ Eval compute in
     Ifopt (IPv4_encoder_impl (initialize_Aligned_ByteString 100) pkt)
   as bs Then IPv4_decoder_impl (fst (fst bs))
         Else None.
-(* This is working now. *)
-Compute
-   match IPv4_decoder_impl bin_pkt with
-   | Some (p, _, _) => Some ((wordToN p.(SourceAddress)), wordToN p.(DestAddress))
-   | None => None
-   end.
-
-Eval compute in onesComplement (Vector.to_list bin_pkt').
-
 (* and it does! *)
 
 (* This should fail because the total length field is too short, *)
@@ -238,3 +231,37 @@ Eval compute in
   as bs Then IPv4_decoder_impl (fst (fst bs))
         Else None.
 (* and it does! *)
+
+(* Some addition checksum sanity checks. *)
+Compute
+   match IPv4_decoder_impl bin_pkt with
+   | Some (p, _, _) => Some ((wordToN p.(SourceAddress)), wordToN p.(DestAddress))
+   | None => None
+   end.
+
+Goal match AlignedIPChecksum.calculate_IPChecksum bin_pkt' 0 ()()  with
+   | Some (p, _, _) => p = bin_pkt
+   | None => True
+   end.
+  reflexivity.
+Qed.
+
+Definition pkt' := {|
+  TotalLength := WO~0~1~1~0~0~1~0~0~0~0~0~0~0~0~0~0;
+  ID := WO~0~0~0~0~0~0~0~0~0~0~0~0~0~0~0~0;
+  DF := false;
+  MF := false;
+  FragmentOffset := WO~0~0~0~0~0~0~0~0~0~0~0~0~0;
+  TTL := WO~0~0~1~0~0~1~1~0;
+  Protocol := Fin.F1;
+  SourceAddress := WO~1~1~0~0~0~0~0~0~1~0~1~0~1~0~0~0~1~1~0~1~1~1~1~0~0~0~0~0~1~0~1~0;
+  DestAddress := WO~1~1~0~0~0~0~0~0~1~0~1~0~1~0~0~0~1~1~0~1~1~1~1~0~0~0~0~0~0~0~0~1;
+  Options := [] |}.
+
+Goal match IPv4_encoder_impl (initialize_Aligned_ByteString 24) pkt'  with
+   | Some (p, _, _) => p = bin_pkt
+   | None => True
+   end.
+  compute.
+  reflexivity.
+Qed.
